Generated/ERC20simple/ERC20Shim/fun_transferFromSimple_user.lean
@@ -13,30 +13,73 @@ section
 
 open Clear EVMState Ast Expr Stmt FunctionDefinition State Interpreter ExecLemmas OutOfFuelLemmas Abstraction YulNotation PrimOps ReasoningPrinciple Utilities ERC20Shim.Common Generated.ERC20simple ERC20Shim
 
-def A_fun_transferFromSimple (var var_1 var_2 : Identifier) (var_from var_to var_value : Literal) (s₀ s₉ : State) : Prop := sorry
+def A_fun_transferFromSimple (var var_1 var_2 : Identifier) (var_from var_to var_value : Literal) (s₀ s₉ : State) : Prop :=
+  let valid := var_value ≤ var_from ∧
+               var_to ≤ var_to + var_value ∧
+               var_from - var_value ≤ var_from
+  ( valid → s₉ = s₀⟦var ↦ 1⟧⟦var_1 ↦ var_from - var_value⟧⟦var_2 ↦ var_to + var_value⟧) ∧
+  (¬valid → s₉ = s₀⟦var ↦ 0⟧⟦var_1 ↦ var_from⟧⟦var_2 ↦ var_to⟧)
 
 set_option maxHeartbeats 400000 in
 lemma fun_transferFromSimple_abs_of_concrete {s₀ s₉ : State} {var var_1 var_2 var_from var_to var_value} :
   Spec (fun_transferFromSimple_concrete_of_code.1 var var_1 var_2 var_from var_to var_value) s₀ s₉ →
   Spec (A_fun_transferFromSimple var var_1 var_2 var_from var_to var_value) s₀ s₉ := by
-  unfold fun_transferFromSimple_concrete_of_code A_fun_transferFromSimple
+  unfold fun_transferFromSimple_concrete_of_code 
   rcases s₀ with ⟨evm, varstore⟩ | _ | _ <;> [simp only; aesop_spec; aesop_spec]
   apply spec_eq
-  rintro h ⟨h₁, ⟨ss, h₂⟩⟩
+  rintro h ⟨s₁, ⟨ss, h₂⟩⟩
   clr_funargs at ss
   clr_varstore ss,
-  rcases h₂ with ⟨w₂, ⟨hw₂, hw₃⟩⟩
-  -- clr_spec at ss
-  -- clr_spec at hw₂
-  apply Spec_ok_unfold at hw₂
+  rcases h₂ with ⟨s₂, ⟨hs₂, ⟨s₃, ⟨hs₃, rest⟩⟩⟩⟩
+  apply Spec_ok_unfold at hs₂
   apply Spec_ok_unfold at ss
   unfold A_if_5295847412656974480 at ss
   clr_varstore ss,
   by_cases eq : (decide (var_from < var_value)).toUInt256 = 0
-  simp [eq] at ss
-  have hss : State.isOk h₁ := by aesop
-  clr_varstore hw₂,
-  clr_varstore hw₃,
+  · simp [eq] at ss
+    have hss : State.isOk s₁ := by aesop
+    apply Spec_ok_unfold at hs₃
+    clr_varstore hs₂,
+    clr_varstore hs₃,
+    dsimp [A_checked_sub_uint256] at hs₂
+    -- Here we're forced to consider overflow. 
+    by_cases eq₁ : s₁["var_from"]!! < s₁["var_from"]!! - (s₁["var_value"]!!)
+    · -- Underflow ocurred.
+      -- Here I spec'd revert as `s.diverge` (i.e. set out of fuel), prolly not smart.
+      sorry
+    · -- No underflow.
+      simp [eq₁] at hs₂
+      have : State.isOk s₂ := by aesop
+      dsimp [A_checked_add_uint256] at hs₃
+      by_cases eq₂ : s₂["var_to"]!! + (s₂["var_value"]!!) < s₂["var_to"]!!
+      · -- Overflow ocurred.
+        -- Reverts????
+        sorry
+      · -- No overflow.
+        simp [eq₂] at hs₃
+        have : State.isOk s₃ := by aesop
+        unfold A_fun_transferFromSimple
+        intros valid
+        -- The only case where valid. I think `eq` is actually "not". It's late.
+        have isValid : valid := sorry
+        refine' ⟨_, (absurd isValid ·)⟩
+        simp [isValid]
+        let s₄ := s₃⟦"expr_component_3"↦s₃["expr_12"]!!⟧⟦"var"↦s₃["expr_6"]!!⟧⟦"var_1"↦s₃["expr_9"]!!⟧⟦"var_2"↦s₃["expr_12"]!!⟧
+        have hs₄ : 🧟(s₄) = s₄ := by aesop_spec
+        have h₁s₄ : s₄.isOk := by aesop
+        rw [hs₄] at rest
+        simp [s₄] at rest
+        have : ∃ evm varstore, s₃ = .Ok evm varstore := by aesop
+        rcases this with ⟨evm, ⟨varstore, hx⟩⟩
+        
+
+
+        
+
+
+  -- simp at hw₅
+  -- clr_varstore hw₅,
+
 
   -- rw [←ss] at hw₂
   -- clr_varstore ss,
