Generated/ERC20simple/ERC20Shim/Common/if_2792370840247009933_user.lean
@@ -11,7 +11,8 @@ section
 
 open Clear EVMState Ast Expr Stmt FunctionDefinition State Interpreter ExecLemmas OutOfFuelLemmas Abstraction YulNotation PrimOps ReasoningPrinciple Utilities Generated.ERC20simple ERC20Shim
 
-def A_if_2792370840247009933 (s₀ s₉ : State) : Prop := sorry
+def A_if_2792370840247009933 (s₀ s₉ : State) : Prop :=
+  (if s₀["_1"]!! = 0 then s₀ else s₀.diverge) = s₉
 
 lemma if_2792370840247009933_abs_of_concrete {s₀ s₉ : State} :
   Spec if_2792370840247009933_concrete_of_code s₀ s₉ →
