Generated/ERC20simple/ERC20Shim/Common/if_668760047301878650_user.lean
@@ -13,6 +13,9 @@ section
 open Clear EVMState Ast Expr Stmt FunctionDefinition State Interpreter ExecLemmas OutOfFuelLemmas Abstraction YulNotation PrimOps ReasoningPrinciple Utilities Generated.ERC20simple ERC20Shim
 
 def A_if_668760047301878650 (s₀ s₉ : State) : Prop := sorry
+  -- s₉ = if s₀["expr_2"]!! = 0
+  --      then s₀
+  --      else s₀⟦"var_newFrom"↦1⟧)
 
 lemma if_668760047301878650_abs_of_concrete {s₀ s₉ : State} :
   Spec if_668760047301878650_concrete_of_code s₀ s₉ →
