Generated/ERC20simple/ERC20Shim/panic_error_0x11_user.lean
@@ -10,11 +10,11 @@ section
 
 open Clear EVMState Ast Expr Stmt FunctionDefinition State Interpreter ExecLemmas OutOfFuelLemmas Abstraction YulNotation PrimOps ReasoningPrinciple Utilities 
 
-def A_panic_error_0x11   (s₀ s₉ : State) : Prop := sorry
+def A_panic_error_0x11 (s₀ s₉ : State) : Prop := sorry
 
 lemma panic_error_0x11_abs_of_concrete {s₀ s₉ : State}  :
   Spec (panic_error_0x11_concrete_of_code.1  ) s₀ s₉ →
-  Spec (A_panic_error_0x11  ) s₀ s₉ := by
+  Spec (A_panic_error_0x11) s₀ s₉ := by
   unfold panic_error_0x11_concrete_of_code A_panic_error_0x11
   sorry
 
